fstar/Hacspec.Chacha20.Proof.fst
@@ -1,0 +1,138 @@
+module Hacspec.Chacha20.Proof
+
+open FStar.Tactics
+open Hacspec.Lib
+open FStar.Mul
+open Hacspec.Chacha20
+
+module S = Spec.Chacha20
+module H = Hacspec.Chacha20
+module LSeq = Lib.Sequence
+module Seq = FStar.Seq
+module LSeqLemmas = Lib.Sequence.Lemmas
+
+module LC = Lib.LoopCombinators
+
+let rec make_list (elem: 'a) (n: nat): list 'a
+  = if n = 0 then [] else elem::make_list elem (n-1)
+
+let unfold_repeat (f: 'a -> 'a) (acc0: 'a) (i:pos)
+  : Lemma (LC.repeat i f acc0 == f (LC.repeat (i - 1) f acc0))
+  = LC.unfold_repeat i f acc0 (i-1) 
+
+#set-options "--fuel 0 --ifuel 0 --z3rlimit 30"
+
+let equiv_line (a b d: state_idx_t) (s: pos {s < 32}) (state: state_t)
+  : Lemma (S.line a b d (pub_u32 s) state == H.chacha20_line a b d s state)
+          [SMTPat (H.chacha20_line a b d s state)]
+  = assert (S.line a b d (pub_u32 s) state `LSeq.equal` H.chacha20_line a b d s state)
+
+let equiv_constants_init
+  : squash (LSeq.map secret S.chacha20_constants == chacha20_constants_init ())
+  = let l = S.([c0;c1;c2;c3]) in
+    assert_norm (FStar.List.Tot.length l == 4);
+    assert_norm S.(let h (i:nat{i<4}) = FStar.List.Tot.index l i in h 0 = c0 /\ h 1 = c1 /\ h 2 = c2 /\ h 3 = c3);
+    LSeq.eq_intro (LSeq.map #_ #_ #(4 <: size_nat) secret S.chacha20_constants) (chacha20_constants_init ())
+
+let equiv_init (key: cha_cha_key_t) (iv: cha_cha_iv_t) (ctr: uint32)
+  : Lemma (S.chacha20_init key iv (v ctr) == H.chacha20_init key iv ctr)
+          [SMTPat (H.chacha20_init key iv ctr)]
+  = ()
+
+let equiv_quarter_round (a b c d: state_idx_t) (state: state_t)
+  : Lemma (S.quarter_round a b c d state == H.chacha20_quarter_round a b c d state)
+          [SMTPat (H.chacha20_quarter_round a b c d state)]
+  = ()
+
+let equiv_double_round (state: state_t)
+  : Lemma (S.double_round state == H.chacha20_double_round state)
+          [SMTPat (H.chacha20_double_round state)]
+  = ()
+
+#push-options "--max_fuel 0 --z3rlimit 15"
+let equiv_rounds (st: state_t)
+  : Lemma (S.rounds st == H.chacha20_rounds st)
+          [SMTPat (H.chacha20_rounds st)]
+  = assert (S.rounds st == chacha20_rounds st) 
+        by (norm [delta_only [`%S.rounds; `%chacha20_rounds]];
+            iter (fun _ -> l_to_r [`unfold_repeat]) (make_list () 10);
+            l_to_r [`LC.eq_repeat0];
+            norm [primops; iota; delta_only [`%usize; `%foldi]; zeta_full])
+#pop-options
+
+let equiv_core (ctr: uint32) (st0: state_t)
+  : Lemma (S.chacha20_core (v ctr) st0 == chacha20_core ctr st0)
+          [SMTPat (H.chacha20_core ctr st0)]
+  = let s0 = st0 in
+    let s1 = array_upd st0 (usize 12) (
+                      (array_index (s0) (usize 12)) +. (ctr)) in
+    let k = H.chacha20_rounds s1 in
+    let ka = k `array_add (+.)` s1 in
+    let kb = k `array_add (+.)` s0 in
+    let kb' = array_upd kb (usize 12) (
+                      (array_index (kb) (usize 12)) +. (ctr)) in
+    assert (u32 (v ctr) == ctr);
+    assert(S.chacha20_add_counter s0 (v ctr) == s1);
+    assert(S.rounds s1 == H.chacha20_rounds s1);
+    assert(S.sum_state k s0 == kb);
+    assert(S.chacha20_add_counter kb (v ctr) == kb');
+    assert(ka == H.chacha20_core ctr st0);
+    assert(kb' == S.chacha20_core (v ctr) st0);
+    assert(forall i. i <> 12 ==> s0.[i] ==  s1.[i]);
+    assert(forall i. i <> 12 ==> ka.[i] ==  kb.[i]);
+    assert(forall i. i <> 12 ==> ka.[i] ==  kb'.[i]);
+    assert(s1.[12] ==  s0.[12] +. ctr);
+    assert(ka.[12] ==  k.[12] +. s1.[12]);
+    assert(kb.[12] ==  k.[12] +. s0.[12]);
+    assert(kb'.[12] ==  k.[12] +. s0.[12] +. ctr);
+    assert(kb'.[12] ==  k.[12] +. (s0.[12] +. ctr));
+    assert(kb'.[12] ==  k.[12] +. s1.[12]);
+    assert(forall i. i >= 0 /\ i < 16 ==> ka.[i] ==  kb'.[i]);
+    LSeq.eq_intro ka kb'
+
+let equiv_key_block (state: state_t)
+  : Lemma (S.chacha20_key_block state == chacha20_key_block state)
+          [SMTPat (H.chacha20_key_block state)]
+  = ()
+
+let equiv_key_block0 (key: cha_cha_key_t) (iv: cha_cha_iv_t)
+  : Lemma (chacha20_key_block0 key iv == S.chacha20_key_block0 key iv)
+          [SMTPat (H.chacha20_key_block0 key iv)]
+  = ()
+
+let equiv_encrypt_block (st0: state_t) (ctr: uint32) (plain: block_t)
+  : Lemma (H.chacha20_encrypt_block st0 ctr plain == S.chacha20_encrypt_block st0 (v ctr) plain)
+          [SMTPat (H.chacha20_encrypt_block st0 ctr plain)]
+  = ()
+
+let equiv_encrypt_last (st0:state_t) (ctr:uint32) (plain: byte_seq {seq_len plain < 64})
+  : Lemma (H.chacha20_encrypt_last st0 ctr plain == S.chacha20_encrypt_last st0 (v ctr) (seq_len plain) plain)
+          [SMTPat (H.chacha20_encrypt_last st0 ctr plain)]
+  = ()
+
+open Hacspec.Lib.FoldiLemmas
+
+let chacha20_update_equiv (st0 : state_t) (cipher : byte_seq) 
+  : Lemma (H.chacha20_update st0 cipher == S.chacha20_update st0 cipher)
+          [SMTPat (H.chacha20_update st0 cipher)]
+  = let blocks_out: seq uint8 = seq_new_ (secret (pub_u8 0x0)) (seq_len cipher) in
+    let n_blocks: uint_size = seq_num_exact_chunks cipher 64 in
+  
+  let f (i: nat {i<n_blocks}) (msg_block: lseq uint8 64): block_t = 
+    chacha20_encrypt_block st0 (secret (pub_u32 i)) (array_from_seq 64 msg_block)
+  in
+  let blocks_out' = map_blocks_foldi #uint8 #(seq_len cipher) 64 n_blocks n_blocks cipher blocks_out f in
+  LSeqLemmas.map_blocks_extensionality 64 cipher (S.chacha20_encrypt_block st0) (S.chacha20_encrypt_last st0) f (S.chacha20_encrypt_last st0);
+  LSeq.lemma_map_blocks 64 cipher f (S.chacha20_encrypt_last st0);
+  map_blocks_foldi_equiv_lemma #uint8 (seq_len cipher) 64 n_blocks n_blocks cipher blocks_out f;
+  LSeq.lemma_map_blocks_multi 64 n_blocks n_blocks (Seq.slice cipher 0 (n_blocks * 64)) f;
+  let last_block: seq uint8 = seq_get_remainder_chunk cipher 64 in
+  assert (S.chacha20_update st0 cipher `LSeq.equal`
+         (if seq_len last_block = 0 then blocks_out'
+          else seq_set_chunk blocks_out' 64 n_blocks (chacha20_encrypt_last st0 (secret (pub_u32 n_blocks)) last_block)))
+
+let chacha20_equiv (key: cha_cha_key_t) (iv: cha_cha_iv_t) (ctr: pub_uint32) (m: byte_seq)
+  : Lemma (S.chacha20_encrypt_bytes key iv (v ctr) m == H.chacha20 key iv ctr m)
+          [SMTPat (H.chacha20 key iv ctr m)]
+  = ()
+
